src/coq/CFGProp.v
@@ -15,6 +15,33 @@ Require Vellvm.AstLib.
 Import ListNotations.
 Open Scope list_scope.
 
+(* invariants of the CFG machine -------------------------------------------- *)
+
+Lemma incr_pc_in_block: forall CFG p1 p2, incr_pc CFG p1 = Some p2 -> (fn p1 = fn p2) /\ (bk p1 = bk p2).
+Proof.
+  intros CFG p1 p2 H.
+  unfold incr_pc in H.
+  destruct p1.
+  destruct (find_function CFG fn); simpl in H; try solve [inversion H].
+  destruct (find_block (blks (df_instrs d)) bk); simpl in H; try solve [inversion H].
+  destruct (block_to_cmd b pt); simpl in H; try solve [inversion H].
+  destruct p. destruct o; try inversion H.
+  simpl. split; reflexivity.
+Qed.  
+
+Lemma find_block_same_fid : forall CFG fid br phis p,
+    find_block_entry CFG fid br = Some (BlockEntry phis p) -> (fn p) = fid.
+Proof.
+  intros CFG fid br phis p H.
+  unfold find_block_entry in H.
+  destruct (find_function CFG fid); simpl in H; try solve [inversion H].
+  destruct (find_block (blks (df_instrs d)) br); simpl in H; try solve [inversion H].
+  destruct b. unfold block_to_entry in H. simpl in H. inversion H.
+  simpl. reflexivity.
+Qed.  
+  
+    
+
 (* syntactic structure ------------------------------------------------------ *)
 
 Inductive CFG_has_code_at (CFG:mcfg) (P:pc -> Prop) : pc -> code -> Prop :=
@@ -64,21 +91,21 @@ Qed.
 Definition CFG_has_pc (CFG:mcfg) (p:pc) : Prop :=
   exists cmd, fetch CFG p = Some cmd.
 
-Definition CFG_fun_has_block_id (CFG:mcfg) (fid:function_id) (bid:block_id) (p:pc) : Prop :=
-  exists phis, find_block_entry CFG fid bid = Some (BlockEntry phis p) /\ CFG_has_pc CFG p. 
+Definition CFG_fun_has_block_id (CFG:mcfg) (fid:function_id) (bid:block_id) phis (p:pc) : Prop :=
+  find_block_entry CFG fid bid = Some (BlockEntry phis p) /\ CFG_has_pc CFG p. 
 
 
 Inductive CFG_fun_has_terminator_lbls (CFG:mcfg) (fid:function_id) : terminator -> Prop :=
 | lbls_Ret : forall v, CFG_fun_has_terminator_lbls CFG fid (TERM_Ret v)
 | lbls_Ret_void : CFG_fun_has_terminator_lbls CFG fid TERM_Ret_void
 | lbls_TERM_Br :
-    forall v br1 p1 br2 p2
-      (Hbr1 : CFG_fun_has_block_id CFG fid br1 p1)
-      (Hbr2 : CFG_fun_has_block_id CFG fid br2 p2),
+    forall v br1 phis1 p1 br2 phis2 p2
+      (Hbr1 : CFG_fun_has_block_id CFG fid br1 phis1 p1)
+      (Hbr2 : CFG_fun_has_block_id CFG fid br2 phis2 p2),
       CFG_fun_has_terminator_lbls CFG fid (TERM_Br v br1 br2)
 | lbls_TERM_Br_1 :
-    forall br p
-      (Hbr : CFG_fun_has_block_id CFG fid br p),
+    forall br phis p
+      (Hbr : CFG_fun_has_block_id CFG fid br phis p),
       CFG_fun_has_terminator_lbls CFG fid (TERM_Br_1 br)
 | lbls_Resume : forall v, CFG_fun_has_terminator_lbls CFG fid (TERM_Resume v)
 .
@@ -99,18 +126,18 @@ Inductive CFG_has_terminator_at (CFG:mcfg) : pc -> instr_id -> terminator -> Pro
       CFG_has_terminator_at CFG p iid t.
 
 
-Inductive CFG_fun_has_block (CFG:mcfg) (fid:function_id) (b:block) : Prop :=
+Inductive CFG_fun_has_block (CFG:mcfg) (fid:function_id) (b:block) phis : Prop :=
 | CFG_fun_has_block_intro:
-    forall phis 
+    forall
       (HFind: find_block_entry CFG fid (blk_id b) = Some (BlockEntry phis (blk_entry_pc fid b)))      
       (Hcode: CFG_has_code_at CFG (fun q => q = blk_term_pc fid b) (blk_entry_pc fid b) (blk_code b))
       (Hterm: CFG_has_terminator_at CFG (blk_term_pc fid b) (blk_term_id b) (blk_terminator b))
     ,
-      CFG_fun_has_block CFG fid b.
+      CFG_fun_has_block CFG fid b phis.
 
 
 Definition CFG_fun_has_blocks (CFG:mcfg) (fid:function_id) (bs:list block) : Prop :=
-  Forall (fun b => CFG_fun_has_block CFG fid b /\ CFG_fun_has_terminator_lbls CFG fid (snd (blk_term b))) bs.
+  Forall (fun b => exists phis, CFG_fun_has_block CFG fid b phis /\ CFG_fun_has_terminator_lbls CFG fid (snd (blk_term b))) bs.
 
 
 (* well formedness ---------------------------------------------------------- *)
